Isabelle2/MultiPaxos.thy
@@ -1,0 +1,214 @@
+theory MultiPaxos
+imports Main  "~~/src/HOL/Library/Monad_Syntax"
+begin
+
+datatype ('v,'a,'b) msg =
+  Phase1a (leader: 'a) (ballot:'b)
+| Phase1b (last_vote:"nat \<Rightarrow> ('v \<times> nat) option") (new_ballot: 'b) (acceptor:'a)
+| Phase2a (inst: nat) (for_ballot:'b) (suggestion:'v) (leader: 'a)
+| Phase2b (inst: nat) (ballot:'b) (acceptor: 'a)
+| Vote (inst: nat) (val: 'v)
+  -- {* Instructs a learner that a value has been decided *}
+| Fwd (val: 'v)
+  -- {* Forwards a proposal to another proposer (the leader) *}
+
+datatype ('v,'a,'b)  packet =
+  -- {* A message with sender/destination information *}
+  Packet (sender: 'a) (dst: 'a) (msg: "('v,'a,'b) msg")
+
+record ('v,'a,'b) mp_state =
+  acceptors :: "'a set"
+    -- {* The set of all acceptors *}
+  ballot :: "'a \<Rightarrow> 'b option"
+    -- {* the highest ballot in which an acceptor participated *}
+  vote :: "'a \<Rightarrow> nat \<Rightarrow> 'v option"
+    -- {* The last vote cast by an acceptor *}
+  last_ballot :: "'a \<Rightarrow> nat \<Rightarrow> 'b option"
+    -- {* For an acceptor a, this is the ballot in which "vote a" was cast *}
+  highest_seen :: "'a \<Rightarrow> 'b option"
+    -- {* highest_seen is used by an acceptor to find a high enough ballot *}
+  onebs :: "'a \<Rightarrow> nat \<Rightarrow> 'b \<Rightarrow> ('a \<times> ('v \<times> 'b) option) list"
+    -- {* For an acceptor a and a ballot b, 
+      this is the list of all the 1b messages receive by a in b *}
+  pending :: "'a \<Rightarrow> nat \<Rightarrow> 'v option"
+    -- {* For an acceptor a, is "Some v" when a has a pending value v.
+      An acceptor may have only one pending proposal. *}
+  twobs :: "'a \<Rightarrow> nat \<Rightarrow> 'b \<Rightarrow> 'a list"
+    -- {* For an acceptor a and a ballot b, 
+      this is the list of all the 2b messages receive by a in b *}
+  decided :: "'a \<Rightarrow> nat \<Rightarrow> 'v option"
+    -- {* For an acceptor a, this is Some v if a has decided v in some ballot *}
+  nxt_instance :: "'a \<Rightarrow> nat"
+    -- {* When a is a leader, the next instance to use. *}
+
+definition init_state :: "'a set \<Rightarrow> ('v,'a,'b) mp_state" where
+  "init_state accs \<equiv> \<lparr>
+    mp_state.acceptors = accs,
+    ballot = (\<lambda> a . None),
+    vote = (\<lambda> a . \<lambda> i . None),
+    last_ballot = (\<lambda> a . \<lambda> i . None),
+    highest_seen = (\<lambda> a . None),
+    onebs = (\<lambda> a . \<lambda> i . \<lambda> b . []),
+    pending = (\<lambda> a . \<lambda> i . None),
+    twobs = (\<lambda> a . \<lambda> i . \<lambda> b . []),
+    decided = (\<lambda> a . \<lambda> i . None),
+    nxt_instance = (\<lambda> a . 0)\<rparr>"
+
+definition one_b_quorum where
+  "one_b_quorum a i b s \<equiv> 2 * length (onebs s a i b) > card (acceptors s)"
+
+definition map_opt where
+  "map_opt ao bo f \<equiv> ao \<bind> (\<lambda> a . bo \<bind> (\<lambda> b . Some (f a b)))"
+
+definition max_opt where
+  -- {* Applies f only if ao and bo are both not None. Wraps the result in an option. 
+    TODO: wouldn't it be better to extend the nat ordering on "nat option"? Using transfer or lifting? *}
+  "max_opt ao bo f \<equiv> (case ao of None \<Rightarrow> (case bo of None \<Rightarrow> None | Some b \<Rightarrow> Some b) |
+    Some a \<Rightarrow> (case bo of None \<Rightarrow> Some a | Some b \<Rightarrow> Some (f a b)))"
+
+definition highest_voted where
+  "highest_voted a i b s \<equiv>
+    let received = onebs s a i b; 
+        filtered = map snd received;
+        max_pair = (\<lambda> x y . if (snd x > snd y) then x else y);
+        max_pairo = (\<lambda> x y . max_opt x y max_pair);
+        init_val = (if filtered = [] then None else (hd filtered))
+    in case (fold max_pairo filtered init_val) of None \<Rightarrow> None | Some (v,b) \<Rightarrow> Some v"
+
+value "let received = [(3,Some (1::int,5)),(10, Some (3,(40::nat)))];
+        filtered = map snd received;
+        max_pair = (\<lambda> x y . if (snd x > snd y) then x else y);
+        max_pairo = (\<lambda> x y . map_opt x y max_pair)
+    in case (fold max_pairo filtered (hd filtered)) of None \<Rightarrow> None | Some (v,b) \<Rightarrow> Some v"
+
+definition suc_bal :: "nat \<Rightarrow> nat \<Rightarrow> nat \<Rightarrow> nat"
+  where "suc_bal a b N \<equiv> (b div N + 1) * N + a"
+
+fun nx_bal where
+  "nx_bal a None N = suc_bal a 0 N"
+| "nx_bal a (Some b) N = suc_bal a b N"
+
+definition one_a_msgs where
+  "one_a_msgs a s \<equiv> 
+    let
+      next_bal = nx_bal a (highest_seen s a) (card (acceptors s));
+      msg_1a = Phase1a a next_bal 
+    in {Packet a b msg_1a | b . b \<in> (acceptors s)}"
+
+definition nr where
+  "nr s \<equiv> card (acceptors s)"
+
+definition leader where
+  "leader s b \<equiv> case b of None \<Rightarrow> 0 | Some b \<Rightarrow> 
+    (b mod (nr s))"
+
+definition propose where 
+  -- {* If leader, then go ahead with 2a, otherwise forward to the leader. TODO: how to choose an instance? 
+    Maintain a list of available instances? or maybe just a variable last_instance will suffice. 
+    How to record the pending command? *}
+  "propose a v s \<equiv>
+    (if (leader s (ballot s a) = a)
+      then (s, {})
+      else (s, {Packet a (leader s (ballot s a)) (Fwd v)}))"
+ 
+fun send_1a where
+  -- {* a tries to become the leader *}
+  "send_1a a s =
+    (let
+        next_bal = nx_bal a (highest_seen s a) (card (acceptors s));
+        msg_1a = Phase1a a next_bal in
+      (s\<lparr>pending := (pending s)(i := (pending s i)(a := Some v)),
+          highest_seen := (highest_seen s)(a := Some next_bal)\<rparr>,
+          {Packet a b msg_1a | b . b \<in> (acceptors s)}))"
+
+fun receive_1a where
+  "receive_1a a (Phase1a l b) s =
+    (let bal = ballot s a in
+      (if (bal = None \<or> ((the bal) < b))
+       then
+          (let
+            to_send = (\<lambda> i . (vote s a i) \<bind> (\<lambda> v . bal \<bind> (\<lambda> b . Some (v, b))));
+            msg_1b = Phase1b to_send b a;
+            packet = Packet a l msg_1b;
+            state = s\<lparr>ballot := (ballot s)(a := Some b),
+                      highest_seen := (highest_seen s)(a := Some b)\<rparr>
+          in
+          (s, {packet}))
+       else (s,{})))"
+| "receive_1a a _ s = (s,{})"
+
+definition test where "test \<equiv> (\<lambda> i . 0::nat)"
+
+export_code test in Scala file "test.scala"
+
+
+text {* Let's assume that we are using TCP, and therefore have no duplicates *}
+fun receive_1b where
+ "receive_1b a (Phase1b last_vs new_bal a2) s N = (
+    if (new_bal = the (ballot s a))
+    then (
+      (let new_onebs = (\<lambda> i . (a2, last_v i) # (onebs s a i)(the (ballot s a)));
+           suggestion = (case (highest_voted a i new_bal s) of None \<Rightarrow> the (pending s a i) | Some v \<Rightarrow> v);
+           msgs =
+           (if (2 * length new_onebs > N)
+            then {Packet a a2 (Phase2a new_bal suggestion a) | a2 . a2 \<in> acceptors s}
+            else {});
+           new_state = s\<lparr>
+            onebs := (onebs s)(a := ((onebs s a)(the (ballot s a) := new_onebs))),
+            pending := (pending s)(a := Some suggestion)\<rparr>
+       in (new_state, msgs)))
+    else (s,{}))"
+| "receive_1b a _ s N = (s, {})"
+
+fun receive_2a where
+  "receive_2a a (Phase2a b v l) s =
+    (let bal = (ballot s a) in
+      (if (bal = Some b)
+      then (s\<lparr>vote := (vote s)(a := Some v)(*, 
+              last_ballot := (last_ballot s)(a := bal)*)\<rparr>, {Packet a l (Phase2b b a)})
+      else (s, {})))"
+| "receive_2a a _ s = (s, {})"
+
+fun receive_2b where
+  "receive_2b a (Phase2b b a2) (s::('v,'a) mp_state) (N::nat) =
+    (let s = 
+      (if (decided s a = None)
+      then 
+        (let new_twobs = a2 # (twobs s a b)
+        in
+          (if (2 * length new_twobs > N) 
+          then 
+            s\<lparr>twobs := (twobs s)(a := (twobs s a)(b := new_twobs)),
+              decided := (decided s)(a := (pending s a))\<rparr>
+          else
+            s\<lparr>twobs := (twobs s)(a := (twobs s a)(b := new_twobs))\<rparr>))
+      else 
+        s)
+    in (s,{}))"
+| "receive_2b a _ s N = (s, {})"
+
+inductive reachable :: "nat set \<Rightarrow> (nat,nat) mp_state \<times> (nat,nat)packet set \<Rightarrow> bool" for replicas where
+  "reachable replicas ((init_state replicas),{})"
+| "\<lbrakk>reachable replicas (s,n); (t,n') = (send_1a a v s)\<rbrakk> \<Longrightarrow> reachable replicas (t,n \<union> n')" 
+| "\<lbrakk>reachable replicas (s,n); p \<in> n; dst p = l; (t,n') = receive_1a l (msg p) s\<rbrakk> \<Longrightarrow> reachable replicas (t,n \<union> n')" 
+| "\<lbrakk>reachable replicas (s,n); p \<in> n; dst p = a; (t,n') = receive_1b a (msg p) s (card replicas)\<rbrakk> \<Longrightarrow> reachable replicas (t,n \<union> n')" 
+| "\<lbrakk>reachable replicas (s,n); p \<in> n; dst p = a; (t,n') = receive_2a a (msg p) s\<rbrakk> \<Longrightarrow> reachable replicas (t,n \<union> n')" 
+| "\<lbrakk>reachable replicas (s,n); p \<in> n; dst p = a; (t,n') = receive_2b a (msg p) s (card replicas)\<rbrakk> \<Longrightarrow> reachable replicas (t,n \<union> n')" 
+
+(* definition decided where
+  "decided s v \<equiv> \<exists> q . q \<subseteq> acceptors s \<and> card q \<ge> (card (acceptors s) div 2) \<and> \<exists> b . \<forall> a \<in> q . " *)
+
+definition decided where
+  "decided s v \<equiv> \<exists> a \<in> acceptors s . mp_state.decided s a = v"
+
+lemma
+  "reachable {0,1} (x,y) \<Longrightarrow> \<forall> v1 v2 . decided x v1 \<and> decided x v2 \<longrightarrow> v1 = v2" 
+    nitpick[card nat=2, show_all, timeout=300, verbose,
+      card "nat list" = 5, card "(nat \<times> nat) option list" = 25, card "(nat \<times> (nat \<times> nat) option) list" = 25, card "nat option" = 3, card "(nat \<times> nat) option" = 25,
+    card "(nat, nat) mp_state \<times> (nat, nat) packet set" = 1000, card "(nat, nat) msg" = 100, card unit = 1, card "(nat, nat) packet" = 100, card "(nat, nat) mp_state" = 100, iter reachable = 1, 
+    bits = 1]
+oops
+
+export_code send_1a receive_1a receive_1b receive_2a receive_2b init_state in Scala file "simplePaxos.scala"
+
+end
